13MachineCode/Disassemble.thy
@@ -9,18 +9,6 @@ primrec register_map :: "memseg \<Rightarrow> reg" where
 | "register_map Stk = R4"
 | "register_map Acc = R5"
 
-primrec register_offset :: "memseg \<Rightarrow> nat" where
-  "register_offset Hp = 0"
-| "register_offset Env = 1"
-| "register_offset Vals = 2"
-| "register_offset Stk = 3"
-| "register_offset Acc = 4"
-
-primrec pseudoreg_size :: "addr_mode \<Rightarrow> nat" where
-  "pseudoreg_size (Reg r) = (if r = Acc then 1 else 4)"
-| "pseudoreg_size (Con k) = 1"
-| "pseudoreg_size (Mem r) = 1"
-
 fun disassemble' :: "assm \<Rightarrow> mach" where
   "disassemble' (AMov (Reg r) (Reg r')) = MOV (register_map r) (register_map r')"
 | "disassemble' (AMov (Reg r) (Con k)) = LDI (register_map r) k"
@@ -43,289 +31,67 @@ fun unmap_mem' :: "nat \<Rightarrow> memseg \<times> nat" where
 | "unmap_mem' (Suc (Suc (Suc 0))) = (Stk, 0)"
 | "unmap_mem' (Suc (Suc (Suc (Suc x)))) = (case unmap_mem' x of (a, b) \<Rightarrow> (a, Suc b))"
 
+primrec register_offset :: "memseg \<Rightarrow> nat" where
+  "register_offset Hp = 0"
+| "register_offset Env = 1"
+| "register_offset Vals = 2"
+| "register_offset Stk = 3"
+| "register_offset Acc = 4"
+
 primrec pseudoreg_map :: "memseg \<times> nat \<Rightarrow> nat" where
   "pseudoreg_map (r, x) = (if r = Acc then x else 4 * x + register_offset r)"
 
 definition unmap_mem :: "(memseg \<times> nat \<Rightarrow> memseg \<times> nat) \<Rightarrow> nat \<Rightarrow> nat" where
-  "unmap_mem m x = pseudoreg_map (m (unmap_mem' x))"
+  "unmap_mem m \<equiv> pseudoreg_map \<circ> m \<circ> unmap_mem'"
 
-primrec inv_register_map :: "(memseg \<Rightarrow> memseg \<times> nat) \<Rightarrow> reg \<Rightarrow> nat" where
-  "inv_register_map rs R1 = pseudoreg_map (rs Hp)"
-| "inv_register_map rs R2 = pseudoreg_map (rs Env)"
-| "inv_register_map rs R3 = pseudoreg_map (rs Vals)"
-| "inv_register_map rs R4 = pseudoreg_map (rs Stk)"
-| "inv_register_map rs R5 = pseudoreg_map (rs Acc)"
+primrec inv_register_map :: "reg \<Rightarrow> memseg" where
+  "inv_register_map R1 = Hp"
+| "inv_register_map R2 = Env"
+| "inv_register_map R3 = Vals"
+| "inv_register_map R4 = Stk"
+| "inv_register_map R5 = Acc"
+
+abbreviation dissassemble_regs :: "(memseg \<Rightarrow> memseg \<times> nat) \<Rightarrow> reg \<Rightarrow> nat" where
+  "dissassemble_regs rs \<equiv> pseudoreg_map \<circ> rs \<circ> inv_register_map"
 
 primrec disassemble_state :: "assm_state \<Rightarrow> mach_state" where
-  "disassemble_state (S\<^sub>a mem rs pc) = MS (inv_register_map rs) (unmap_mem mem) pc"
-
-primrec dissassembleable :: "assm_state \<Rightarrow> nat \<Rightarrow> bool" where
-  "dissassembleable (S\<^sub>a mem rs pc) lcd = (pc < lcd)"
-
-lemma [dest]: "R1 = register_map r \<Longrightarrow> r = Hp"
-  by (induction r) simp_all
-
-lemma [dest]: "R2 = register_map r \<Longrightarrow> r = Env"
-  by (induction r) simp_all
-
-lemma [dest]: "R3 = register_map r \<Longrightarrow> r = Vals"
-  by (induction r) simp_all
-
-lemma [dest]: "R4 = register_map r \<Longrightarrow> r = Stk"
-  by (induction r) simp_all
-
-lemma [dest]: "R5 = register_map r \<Longrightarrow> r = Acc"
-  by (induction r) simp_all
-
-lemma unmap_times_4 [simp]: "unmap_mem' (4 * k) = (Hp, k)"
-  by (induction k) (simp_all add: numeral_def)
-
-lemma [simp]: "unmap_mem' (k * 4) = (Hp, k)"
-  by (induction k) (simp_all add: numeral_def)
-
-lemma [simp]: "unmap_mem' (Suc (k * 4)) = (Env, k)"
-  by (induction k) (simp_all add: numeral_def)
-
-lemma [simp]: "unmap_mem' (Suc (Suc (k * 4))) = (Vals, k)"
-  by (induction k) (simp_all add: numeral_def)
-
-lemma [simp]: "unmap_mem' (k * 4 + 3) = (Stk, k)"
-  by (induction k) (simp_all add: numeral_def)
-
-lemma [simp]: "unmap_mem' p = (a, b) \<Longrightarrow> unmap_mem' (4 + p) = (a, Suc b)"
-  by (simp add: numeral_def)
+  "disassemble_state (S\<^sub>a mem rs pc) = MS (dissassemble_regs rs) (unmap_mem mem) pc"
 
 lemma [simp]: "length (disassemble cd) = length cd"
   by (simp add: disassemble_def)
 
-lemma [dest]: "unmap_mem' x = (Hp, ps Hp) \<Longrightarrow> x = ps Hp * 4"
-  by (induction x arbitrary: ps rule: unmap_mem'.induct) (auto split: prod.splits)
-
-lemma [dest]: "unmap_mem' x = (Env, ps Env) \<Longrightarrow> x = Suc (ps Env * 4)"
-  by (induction x arbitrary: ps rule: unmap_mem'.induct) (auto split: prod.splits)
-
-lemma [dest]: "unmap_mem' x = (Vals, ps Vals) \<Longrightarrow> x = Suc (Suc (ps Vals * 4))"
-  by (induction x arbitrary: ps rule: unmap_mem'.induct) (auto split: prod.splits)
-
-lemma [dest]: "unmap_mem' x = (Stk, ps Stk) \<Longrightarrow> x = Suc (Suc (Suc (ps Stk * 4)))"
-  by (induction x arbitrary: ps rule: unmap_mem'.induct) (auto split: prod.splits)
-
-lemma [dest]: "unmap_mem' x = (Acc, b) \<Longrightarrow> False"
-  by (induction x arbitrary: b rule: unmap_mem'.induct) (auto split: prod.splits)
-
-lemma [simp]: "unmap_mem' 2 = (Vals, 0)"
-  by (simp add: numeral_def)
-
-lemma [simp]: "unmap_mem' (16 + 16 * x) = (Hp, 4 + 4 * x)"
-proof -
-  have "unmap_mem' (4 * (4 * Suc x)) = (Hp, 4 * Suc x)" by (metis unmap_times_4)
-  thus ?thesis by simp
-qed
-
-(*
-lemma [simp]: "r \<noteq> Acc \<Longrightarrow> unmap_mem' (inv_register_map ps act (register_map r)) = (r, ps r)"
+lemma [simp]: "inv_register_map (register_map r) = r"
   by (induction r) simp_all
 
-lemma inv_reg_map_reg: "r \<noteq> Acc \<Longrightarrow>
-  (inv_register_map ps act)(R5 := inv_register_map ps act (register_map r)) = 
-    inv_register_map (ps(Acc := ps r)) r"
-proof
-  fix x
-  assume "r \<noteq> Acc"
-  thus "((inv_register_map ps act)(R5 := inv_register_map ps act (register_map r))) x = 
-      inv_register_map (ps(Acc := ps r)) r x"
-  proof (induction x)
-    case R5
-    thus ?case by (induction r) simp_all
-  qed simp_all
-qed
+lemma [simp]: "register_map (inv_register_map r) = r"
+  by (induction r) simp_all
 
-lemma inv_reg_map_none: "(inv_register_map ps act)(R5 := k) = inv_register_map (ps(Acc := k)) Acc"
-proof
-  fix x
-  show "((inv_register_map ps act)(R5 := k)) x = inv_register_map (ps(Acc := k)) Acc x"
-    by (induction x) simp_all
-qed
+lemma [dest]: "inv_register_map r = Acc \<Longrightarrow> r = R5"
+  by (induction r) simp_all
 
-lemma [simp]: "(inv_register_map ps act)
-    (R5 := if act = Acc then ps Acc else 4 * ps Acc + register_offset act) = inv_register_map ps act"
-  by auto
+lemma [simp]: "unmap_mem' (4 * y) = (Hp, y)" 
+  by (induction y) (simp_all add: numeral_def)
 
-lemma [simp]: "m \<noteq> Acc \<Longrightarrow> unmap_mem' (4 * k + register_offset m) = (m, k)"
-proof (induction k)
-  case 0
-  thus ?case by (induction m) (simp_all add: numeral_def)
-qed (simp_all add: numeral_def)
+lemma [simp]: "unmap_mem' (Suc (4 * y)) = (Env, y)" 
+  by (induction y) (simp_all add: numeral_def)
 
-lemma [simp]: "r \<noteq> Acc \<Longrightarrow> inv_register_map (ps(r := k)) act R5 = inv_register_map ps act R5"
-  by (induction act) simp_all
+lemma [simp]: "unmap_mem' (Suc (Suc (4 * y))) = (Vals, y)" 
+  by (induction y) (simp_all add: numeral_def)
 
-lemma [simp]: "r \<noteq> Acc \<Longrightarrow> inv_register_map (ps(r := ps r + k)) act = 
-  ((inv_register_map ps act) (register_map r := inv_register_map ps act (register_map r) + 4 * k))"
-proof
-  fix x
-  assume "r \<noteq> Acc"
-  thus "inv_register_map (ps(r := ps r + k)) act x =
-    ((inv_register_map ps act) 
-      (register_map r := inv_register_map ps act (register_map r) + 4 * k)) x" 
-    by (induction x) auto
-qed
+lemma [simp]: "unmap_mem' (4 * y + 3) = (Stk, y)" 
+  by (induction y) (simp_all add: numeral_def)
 
-lemma [simp]: "r \<noteq> Acc \<Longrightarrow> (inv_register_map ps r) (R5 := 4 * ps Acc + register_offset r + 4 * k) = 
-  inv_register_map (ps(Acc := ps Acc + k)) r"
-proof
-  fix x
-  assume "r \<noteq> Acc"
-  thus "((inv_register_map ps r) (R5 := 4 * ps Acc + register_offset r + 4 * k)) x =
-    inv_register_map (ps(Acc := ps Acc + k)) r x" by (induction x) simp_all
-qed
+lemma [dest]: "unmap_mem' x = (Acc, y) \<Longrightarrow> False"
+  by (induction x arbitrary: y rule: unmap_mem'.induct) (auto split: prod.splits)
 
-lemma [simp]: "ps r \<ge> k \<Longrightarrow> r \<noteq> Acc \<Longrightarrow>
-  inv_register_map (ps(r := ps r - k)) act = ((inv_register_map ps act)
-    (register_map r := inv_register_map ps act (register_map r) - 4 * k))"
-proof
-  fix x
-  assume "ps r \<ge> k" and "r \<noteq> Acc"
-  thus "inv_register_map (ps(r := ps r - k)) act x =
-    ((inv_register_map ps act) 
-      (register_map r := inv_register_map ps act (register_map r) - 4 * k)) x" 
-    by (induction x) auto
-qed
+lemma [simp]: "pseudoreg_map (unmap_mem' x) = x"
+  by (induction x rule: unmap_mem'.induct) (auto split: prod.splits)
 
-lemma [simp]: "ps Acc \<ge> k \<Longrightarrow> r \<noteq> Acc \<Longrightarrow>
-  (inv_register_map ps r) (R5 := 4 * ps Acc + register_offset r - 4 * k) = 
-    inv_register_map (ps(Acc := ps Acc - k)) r"
-proof
-  fix x
-  assume "ps Acc \<ge> k" and "r \<noteq> Acc"
-  thus "((inv_register_map ps r) (R5 := 4 * ps Acc + register_offset r - 4 * k)) x = 
-      inv_register_map (ps(Acc := ps Acc - k)) r x" 
-    by (induction x) simp_all
-qed
+lemma [simp]: "x \<noteq> Acc \<Longrightarrow> unmap_mem' (4 * y + register_offset x) = (x, y)"
+  by (induction x) simp_all
 
-lemma [simp]: "r \<noteq> Acc \<Longrightarrow> unmap_mem mem (inv_register_map ps r (register_map r)) = 
-    pseudoreg_map (mem r (ps r))"
-  by (induction r) (simp_all add: unmap_mem_def split: prod.splits)
-
-lemma [simp]: "r \<noteq> Acc \<Longrightarrow> mem r (ps r) = (t, b) \<Longrightarrow> 
-  (inv_register_map ps act)(R5 := unmap_mem mem (inv_register_map ps act (register_map r))) = 
-    inv_register_map (ps(Acc := b)) t"
-proof
-  fix x
-  assume "mem r (ps r) = (t, b)" and "r \<noteq> Acc"
-  thus "((inv_register_map ps act)(R5 := 
-    unmap_mem mem (inv_register_map ps act (register_map r)))) x = 
-      inv_register_map (ps(Acc := b)) t x"
-  proof (induction x)
-    case R5
-    thus ?case by (induction r) (simp_all add: unmap_mem_def)
-  qed simp_all
-qed
-
-lemma unmap_upd_k: "r \<noteq> Acc \<Longrightarrow> (unmap_mem mem)(inv_register_map ps act (register_map r) := k) = 
-    unmap_mem (mem_upd mem r (ps r) (Acc, k))"
-  by (rule, induction r) (auto simp add: unmap_mem_def split: prod.splits)
-
-lemma [simp]: "r \<noteq> Acc \<Longrightarrow> r' \<noteq> Acc \<Longrightarrow> ((unmap_mem mem)
-  (inv_register_map ps act (register_map r) := inv_register_map ps act (register_map r'))) = 
-    unmap_mem (mem_upd mem r (ps r) (r', ps r'))"
-proof
-  fix x
-  assume "r \<noteq> Acc" and "r' \<noteq> Acc"
-  thus "((unmap_mem mem)
-    (inv_register_map ps act (register_map r) := inv_register_map ps act (register_map r'))) x = 
-      unmap_mem (mem_upd mem r (ps r) (r', ps r')) x"
-  proof (induction r)
-    case Hp
-    thus ?case by (induction r') (auto simp add: unmap_mem_def split: prod.splits)
-  next
-    case Env
-    thus ?case by (induction r') (auto simp add: unmap_mem_def split: prod.splits)
-  next
-    case Vals
-    thus ?case by (induction r') (auto simp add: unmap_mem_def split: prod.splits)
-  next
-    case Stk
-    thus ?case by (induction r') (auto simp add: unmap_mem_def split: prod.splits)
-  qed simp_all
-qed
-
-lemma [simp]: "r \<noteq> Acc \<Longrightarrow> ((unmap_mem mem)(inv_register_map ps act (register_map r) := 
-  (if act = Acc then a else 4 * a + register_offset act))) = 
-    unmap_mem (mem_upd mem r (ps r) (act, a))"
-proof
-  fix x
-  assume "r \<noteq> Acc"
-  thus "((unmap_mem mem)(inv_register_map ps act (register_map r) := 
-    (if act = Acc then a else 4 * a + register_offset act))) x = 
-      unmap_mem (mem_upd mem r (ps r) (act, a)) x"
-        by (induction r) (auto simp add: unmap_mem_def split: prod.splits)
-qed
-
-lemma [simp]: "m \<noteq> Acc \<Longrightarrow> mem m (ps Acc) = (t, b) \<Longrightarrow>  
-  ((inv_register_map ps m)(R5 := unmap_mem mem (4 * ps Acc + register_offset m))) = 
-    inv_register_map (ps(Acc := b)) t"
-proof 
-  fix x
-  assume "mem m (ps Acc) = (t, b)" and "m \<noteq> Acc"
-  thus "((inv_register_map ps m)(R5 := unmap_mem mem (4 * ps Acc + register_offset m))) 
-    x = inv_register_map (ps(Acc := b)) t x"
-      by (induction x) (auto simp add: unmap_mem_def)
-qed
-
-lemma [simp]: "mem act (ps Acc) = (r, b) \<Longrightarrow> r \<noteq> Acc \<Longrightarrow> act \<noteq> Acc \<Longrightarrow>
-  ((inv_register_map ps act)(register_map r := unmap_mem mem (4 * ps Acc + register_offset act))) =
-    (inv_register_map (ps(r := b)) act)"
-proof 
-  fix x
-  assume "mem act (ps Acc) = (r, b)" and "act \<noteq> Acc" and "r \<noteq> Acc"
-  thus "((inv_register_map ps act)
-    (register_map r := unmap_mem mem (4 * ps Acc + register_offset act))) x =
-      (inv_register_map (ps(r := b)) act) x"
-    by (induction x) (auto simp add: unmap_mem_def)
-qed
-
-lemma [simp]: "mem r' (ps r') = (r, b) \<Longrightarrow> r' \<noteq> Acc \<Longrightarrow> r \<noteq> Acc \<Longrightarrow>
-  ((inv_register_map ps act) 
-    (register_map r := unmap_mem mem (inv_register_map ps act (register_map r')))) =
-      (inv_register_map (ps(r := b)) act)"
-proof 
-  fix x
-  assume "mem r' (ps r') = (r, b)" and "r' \<noteq> Acc" and "r \<noteq> Acc"
-  thus "((inv_register_map ps act)
-    (register_map r := unmap_mem mem (inv_register_map ps act (register_map r')))) x =
-      (inv_register_map (ps(r := b)) act) x"
-  proof (induction x)
-    case R1
-    thus ?case by (induction r) (simp_all add: unmap_mem_def)
-  next
-    case R2
-    thus ?case by (induction r) (simp_all add: unmap_mem_def)
-  next
-    case R3
-    thus ?case by (induction r) (simp_all add: unmap_mem_def)
-  next
-    case R4
-    thus ?case by (induction r) (simp_all add: unmap_mem_def)
-  next
-    case R5
-    thus ?case by (induction r) (simp_all add: unmap_mem_def)
-  qed 
-qed
-
-lemma [simp]: "
-  (inv_register_map ps act)(register_map r := inv_register_map ps act (register_map r')) = 
-    (inv_register_map (ps(r := ps r')) (if r = Acc then reg_merge r' act else act))"
-proof
-  fix x
-  show "((inv_register_map ps act)(register_map r := inv_register_map ps act (register_map r'))) x = 
-    (inv_register_map (ps(r := ps r')) (if r = Acc then reg_merge r' act else act)) x" 
-    apply (induction r)
-    apply simp_all
-
-
-lemma [simp]: "(inv_register_map ps act)(R5 := pseudoreg_map (act, ps Acc)) = inv_register_map ps act"
-  by auto
+lemma [simp]: "fst x \<noteq> Acc \<Longrightarrow> unmap_mem' (pseudoreg_map x) = x"
+  by (cases x) simp_all
 
 lemma lookup_disassemble [simp]: "lookup cd pc = Some op \<Longrightarrow> disassemble cd ! pc = disassemble' op"
 proof (induction cd)
@@ -333,47 +99,109 @@ proof (induction cd)
   thus ?case by (induction pc) (simp_all add: disassemble_def)
 qed simp_all
 
-theorem correctm [simp]: "cd\<^sub>a \<tturnstile> \<Sigma>\<^sub>a \<leadsto>\<^sub>a \<Sigma>\<^sub>a' \<Longrightarrow> 
+lemma [simp]: "dissassemble_regs (ps(Acc := (Acc, 0))) = (dissassemble_regs ps)(R5 := 0)"
+  by rule auto
+
+lemma [simp]: "dissassemble_regs (ps(r := ps r')) = 
+    (dissassemble_regs ps)(register_map r := dissassemble_regs ps (register_map r'))"
+  by rule auto
+
+lemma [simp]: "dissassemble_regs (ps(r := (Acc, k))) = (dissassemble_regs ps)(register_map r := k)"
+  by rule auto
+
+lemma [simp]: "fst (ps r') \<noteq> Acc \<Longrightarrow> (dissassemble_regs (ps(r := mem (ps r')))) = 
+    ((dissassemble_regs ps)
+      (register_map r := unmap_mem mem (dissassemble_regs ps (register_map r'))))"
+  by rule (auto simp add: unmap_mem_def)
+
+lemma unmap_mem_with_reg [simp]: "fst r \<noteq> Acc \<Longrightarrow> 
+    ((unmap_mem mem)(pseudoreg_map r := pseudoreg_map r')) = unmap_mem (mem(r := r'))"
+  by rule (auto simp add: unmap_mem_def)
+
+lemma unmap_mem_with_const [simp]: "fst r \<noteq> Acc \<Longrightarrow>
+    ((unmap_mem mem)(pseudoreg_map r := n)) = unmap_mem (mem(r := (Acc, n)))"
+  by rule (auto simp add: unmap_mem_def)
+
+lemma [simp]: "r' \<noteq> Acc \<Longrightarrow> y \<ge> k \<Longrightarrow> 
+  ((dissassemble_regs ps)(register_map r := 4 * y + register_offset r' - 4 * k)) = 
+    (dissassemble_regs (ps(r := (r', y - k))))"
+  by rule auto
+
+lemma [simp]: "r' \<noteq> Acc \<Longrightarrow> 
+  ((dissassemble_regs ps)(register_map r := 4 * y + register_offset r' + 4 * k)) = 
+    (dissassemble_regs (ps(r := (r', y + k))))"
+  by rule auto
+
+theorem correctm [simp]: "cd\<^sub>a \<tturnstile> \<Sigma>\<^sub>a \<leadsto>\<^sub>a \<Sigma>\<^sub>a' \<Longrightarrow>
   disassemble cd\<^sub>a \<tturnstile> disassemble_state \<Sigma>\<^sub>a \<leadsto>\<^sub>m disassemble_state \<Sigma>\<^sub>a'"
 proof (induction \<Sigma>\<^sub>a)
-  case (S\<^sub>a mem ps act pc)
+  case (S\<^sub>a mem ps pc)
   moreover then obtain pc' where P: "pc = Suc pc'" by (simp split: nat.splits)
   ultimately show ?case 
   proof (cases "lookup cd\<^sub>a pc'")
     case (Some op)
-    with S\<^sub>a P have "assm_step mem ps act pc' op = Some \<Sigma>\<^sub>a'" by simp
+    with S\<^sub>a P have "assm_step mem ps pc' op = Some \<Sigma>\<^sub>a'" by simp
     with P Some show ?thesis 
-    proof (induction mem ps act pc' op rule: assm_step.induct)
-      case (1 mem ps act pc' r r')
-      hence "disassemble cd\<^sub>a \<tturnstile> MS (inv_register_map ps act) (unmap_mem mem) (Suc pc') \<leadsto>\<^sub>m 
-        MS ((inv_register_map ps act)(register_map r := inv_register_map ps act (register_map r'))) 
-          (unmap_mem mem) pc'" by simp
-
-      hence "disassemble cd\<^sub>a \<tturnstile> MS (inv_register_map ps act) (unmap_mem mem) (Suc pc') \<leadsto>\<^sub>m 
-        MS (inv_register_map (ps(r := ps r')) (if r = Acc then reg_merge r' act else act)) 
-          (unmap_mem mem) pc'" by simp
-      with 1(1, 3) show ?case by auto
+    proof (induction mem ps pc' op rule: assm_step.induct)
+      case (1 mem ps pc' r r')
+      hence "disassemble cd\<^sub>a ! pc' = MOV (register_map r) (register_map r')" by simp
+      hence "disassemble cd\<^sub>a \<tturnstile> MS (dissassemble_regs ps) (unmap_mem mem) (Suc pc') \<leadsto>\<^sub>m 
+        MS ((dissassemble_regs ps)(register_map r := dissassemble_regs ps (register_map r'))) (unmap_mem mem) pc'" 
+          by (metis evm_mov)
+      with 1 show ?case by auto
     next
-      case (2 mem ps act pc' r k)
-      then show ?case by simp
+      case (2 mem ps pc' r n)
+      hence "disassemble cd\<^sub>a ! pc' = LDI (register_map r) n" by simp
+      hence "disassemble cd\<^sub>a \<tturnstile> MS (dissassemble_regs ps) (unmap_mem mem) (Suc pc') \<leadsto>\<^sub>m 
+        MS ((dissassemble_regs ps)(register_map r := n)) (unmap_mem mem) pc'" 
+          by (metis evm_ldi)
+        with 2 show ?case by auto
+     next
+      case (3 mem ps pc' r r')
+      hence "disassemble cd\<^sub>a ! pc' = LOD (register_map r) (register_map r')" by simp
+      hence "disassemble cd\<^sub>a \<tturnstile> MS (dissassemble_regs ps) (unmap_mem mem) (Suc pc') \<leadsto>\<^sub>m 
+        MS ((dissassemble_regs ps)(register_map r := 
+          unmap_mem mem (dissassemble_regs ps (register_map r')))) (unmap_mem mem) pc'" 
+        by (metis evm_lod)
+      with 3 show ?case by (auto split: if_splits)
     next
-      case (3 mem ps act pc' r r')
-      then show ?case by simp
+      case (5 mem ps pc' r r')
+      hence "disassemble cd\<^sub>a ! pc' = STO (register_map r) (register_map r')" by simp
+      hence "disassemble cd\<^sub>a \<tturnstile> MS (dissassemble_regs ps) (unmap_mem mem) (Suc pc') \<leadsto>\<^sub>m 
+        MS (dissassemble_regs ps) ((unmap_mem mem)(dissassemble_regs ps (register_map r) := 
+          dissassemble_regs ps (register_map r'))) pc'" 
+        by (metis evm_sto)
+      with 5 show ?case by (auto simp del: unmap_mem_with_const split: if_splits)
     next
-      case (5 mem ps act pc' r r')
-      then show ?case by simp
+      case (6 mem ps pc' r n)
+      hence "disassemble cd\<^sub>a ! pc' = STI (register_map r) n" by simp
+      hence "disassemble cd\<^sub>a \<tturnstile> MS (dissassemble_regs ps) (unmap_mem mem) (Suc pc') \<leadsto>\<^sub>m 
+        MS (dissassemble_regs ps) ((unmap_mem mem)(dissassemble_regs ps (register_map r) := n)) pc'" 
+          by (metis evm_sti)
+      with 6 show ?case by (auto split: if_splits)
     next
-      case (6 mem ps act pc' r k)
-      then show ?case by simp
+      case (8 mem ps pc' r k)
+      hence "disassemble cd\<^sub>a ! pc' = SUB (register_map r) (4 * k)" by simp
+      moreover from 8 have "dissassemble_regs ps (register_map r) \<ge> 4 * k" 
+        by (simp split: prod.splits if_splits)
+      ultimately have "disassemble cd\<^sub>a \<tturnstile> MS (dissassemble_regs ps) (unmap_mem mem) (Suc pc') \<leadsto>\<^sub>m 
+        MS ((dissassemble_regs ps)(register_map r := dissassemble_regs ps (register_map r) - 4 * k)) 
+          (unmap_mem mem) pc'" by (metis evm_sub)
+      with 8 show ?case by (auto split: prod.splits if_splits)
     next
-      case (8 mem ps act pc' r k)
-      then show ?case by simp
+      case (9 mem ps pc' r k)
+      hence "disassemble cd\<^sub>a ! pc' = ADD (register_map r) (4 * k)" by simp
+      hence "disassemble cd\<^sub>a \<tturnstile> MS (dissassemble_regs ps) (unmap_mem mem) (Suc pc') \<leadsto>\<^sub>m 
+        MS ((dissassemble_regs ps)(register_map r := dissassemble_regs ps (register_map r) + 4 * k)) 
+          (unmap_mem mem) pc'" by (metis evm_add)
+      with 9 show ?case by (auto split: prod.splits if_splits)
     next
-      case (9 mem ps act pc' r k)
-      then show ?case by simp
-    next
-      case (10 mem ps act pc')
-      then show ?case by simp
+      case (10 mem ps pc')
+      hence "disassemble cd\<^sub>a ! pc' = JMP R5" by simp
+      hence "disassemble cd\<^sub>a \<tturnstile> MS (dissassemble_regs ps) (unmap_mem mem) (Suc pc') \<leadsto>\<^sub>m 
+        MS ((dissassemble_regs ps)(R5 := 0)) (unmap_mem mem) ((dissassemble_regs ps) R5)" 
+          by (metis evm_jmp)
+      with 10 show ?case by (auto split: if_splits split: prod.splits)
     qed simp_all
   qed simp_all
 qed
@@ -382,33 +210,19 @@ theorem correctm_iter [simp]: "iter (\<tturnstile> cd\<^sub>a \<leadsto>\<^sub>a
     iter (\<tturnstile> disassemble cd\<^sub>a \<leadsto>\<^sub>m) (disassemble_state \<Sigma>\<^sub>a) (disassemble_state \<Sigma>\<^sub>a')"
   by (induction \<Sigma>\<^sub>a \<Sigma>\<^sub>a' rule: iter.induct) (simp, metis correctm iter_append iter_one)
 
-lemma [simp]: "inv_register_map (case_memseg 0 0 0 2 0) Acc = case_reg 0 1 2 11 0" 
-  by (auto split: reg.splits)
+lemma [simp]: "dissassemble_regs (case_memseg (Hp, 0) (Env, 0) (Vals, 0) (Stk, 2) (Acc, 0)) = 
+    case_reg 0 (Suc 0) 2 11 0"
+  by (auto split: memseg.splits reg.splits)
 
-lemma [simp]: "inv_register_map (case_memseg hp ep (Suc 0) 0 0) Acc = 
-    case_reg (4 * hp) (Suc (4 * ep)) 6 3 0"
-  by (auto split: reg.splits)
+lemma [simp]: "dissassemble_regs (case_memseg (Hp, x) (Env, y) (Vals, Suc 0) (Stk, 0) (Acc, 0)) =
+    case_reg (4 * x) (Suc (4 * y)) 6 3 0"
+  by (auto split: memseg.splits reg.splits)
 
 lemma [dest]: "unmap_mem' x = (r, y) \<Longrightarrow> x = 4 * y + register_offset r"
   by (induction x arbitrary: y rule: unmap_mem'.induct) (simp_all split: prod.splits)
 
-*)
-
 lemma [simp]: "unmap_mem (case_prod (case_memseg (\<lambda>x. (Acc, 0)) (\<lambda>x. (Acc, 0)) (\<lambda>x. (Acc, 0)) 
-  ((\<lambda>x. (Acc, 0)) (0 := (Acc, 0), Suc 0 := (Env, 0))) undefined)) = (\<lambda>x. 0)(7 := 1)"
-proof (rule, unfold unmap_mem_def)
-  fix x
-  obtain r p where R: "unmap_mem' x = (r, p)" by fastforce
-  moreover hence "x = 4 * p + register_offset r" by auto
-  ultimately have "pseudoreg_map ((case r of 
-        Stk \<Rightarrow> (\<lambda>x. (Acc, 0))(0 := (Acc, 0), Suc 0 := (Env, 0))
-      | Acc \<Rightarrow> undefined 
-      | _ \<Rightarrow> (\<lambda>x. (Acc, 0))) p) = ((\<lambda>x. 0)(3 := 0, 7 := 1)) x" 
-    by (induction r) (simp_all, presburger+, auto)
-  with R show "(case unmap_mem' x of (r, p) \<Rightarrow> 
-    pseudoreg_map (case_prod (case_memseg (\<lambda>x. (Acc, 0)) (\<lambda>x. (Acc, 0)) (\<lambda>x. (Acc, 0))
-      ((\<lambda>x. (Acc, 0))(0 := (Acc, 0), Suc 0 := (Env, 0))) undefined r p))) =
-        ((\<lambda>x. 0)(7 := 1)) x" by simp
-qed
+    ((\<lambda>x. (Acc, 0)) (0 := (Acc, 0), Suc 0 := (Env, 0))) undefined)) = (\<lambda>x. 0)(7 := 1)"
+  by rule (auto simp add: numeral_def unmap_mem_def split: prod.splits memseg.splits)
 
 end
